theories/iris/logrel/fundamental.v
@@ -88,12 +88,12 @@ Section Fundamental.
   Qed.
 
   (* useful lemma for proving compat lemmas for instructions erased by the compiler. *)
-  Lemma sem_type_erased M F L wl ψ τs1 τs2 : 
+  Lemma sem_type_erased M F L WT WL ψ τs1 τs2 :
     ψ = InstrT τs1 τs2 ->
     ⊢ (∀ se s__mem s__rep s__size vs,
           values_interp rti sr se (map (subst_type s__mem s__rep s__size VarT) τs1) vs -∗
           values_interp rti sr se (map (subst_type s__mem s__rep s__size VarT) τs2) vs) -∗
-      have_instruction_type_sem rti sr mr M F L wl [] ψ L.
+      have_instruction_type_sem rti sr mr M F L WT WL [] ψ L.
   Proof.
     iIntros (->) "Hcast".
     iIntros (s__mem s__rep s__size se inst fr lh rvs vs Hsubst) "Hinst Hctx Hrvs Hvs Hfr Hf Hrun".
@@ -105,12 +105,12 @@ Section Fundamental.
     by iApply "Hcast".
   Qed.
 
-  Lemma sem_type_erased_nop M F L wl ψ τs1 τs2 : 
+  Lemma sem_type_erased_nop M F L WT WL ψ τs1 τs2 :
     ψ = InstrT τs1 τs2 ->
     ⊢ (∀ se s__mem s__rep s__size vs,
           values_interp rti sr se (map (subst_type s__mem s__rep s__size VarT) τs1) vs -∗
           ▷values_interp rti sr se (map (subst_type s__mem s__rep s__size VarT) τs2) vs) -∗
-      have_instruction_type_sem rti sr mr M F L wl [AI_basic BI_nop] ψ L.
+      have_instruction_type_sem rti sr mr M F L WT WL [AI_basic BI_nop] ψ L.
   Proof.
     iIntros (->) "Hcast".
     iIntros (s__mem s__rep s__size se inst fr lh rvs vs Hsubst) "Hinst Hctx Hrvs Hvs Hfr Hf Hrun".
@@ -145,7 +145,7 @@ Section Fundamental.
     - iExists _.
       iSplit; done.
   Qed.
-  
+
   Lemma values_interp_one_eq se τ vs :
     values_interp rti sr se [τ] vs ⊣⊢ value_interp rti sr se τ (SValues vs).
   Proof.
@@ -167,17 +167,18 @@ Section Fundamental.
         by iApply big_sepL2_nil.
   Qed.
 
-  Lemma compat_nop M F L wt wt' wl wl' wlf es' :
+  Lemma compat_nop M F L wt wt' wtf wl wl' wlf es' :
     let fe := fe_of_context F in
+    let WT := wt ++ wt' ++ wtf in
+    let WL := wl ++ wl' ++ wlf in
     let ψ := InstrT [] [] in
     has_instruction_type_ok F ψ L ->
     run_codegen (compile_instr mr fe (INop ψ)) wt wl = inr ((), wt', wl', es') ->
-    ⊢ have_instruction_type_sem rti sr mr M F L (wl ++ wl' ++ wlf) (to_e_list es') ψ L.
+    ⊢ have_instruction_type_sem rti sr mr M F L WT WL (to_e_list es') ψ L.
   Proof.
     (* This is currently following the compat_copy lemma very closely *)
-    intros fe ψ Hok Hcompile.
+    intros fe WT WL ψ Hok Hcompile.
     inv_cg_emit Hcompile; subst.
-    rewrite app_nil_l.
     unfold have_instruction_type_sem.
     destruct ψ eqn:Hψ.
     inversion Hψ; subst l l0.
@@ -202,11 +203,13 @@ Section Fundamental.
       iFrame; auto.
   Qed.
 
-  Lemma compat_unreachable M F L L' wt wt' wl wl' wlf ψ es' :
+  Lemma compat_unreachable M F L L' wt wt' wtf wl wl' wlf ψ es' :
     let fe := fe_of_context F in
+    let WT := wt ++ wt' ++ wtf in
+    let WL := wl ++ wl' ++ wlf in
     has_instruction_type_ok F ψ L' ->
     run_codegen (compile_instr mr fe (IUnreachable ψ)) wt wl = inr ((), wt', wl', es') ->
-    ⊢ have_instruction_type_sem rti sr mr M F L (wl ++ wl' ++ wlf) (to_e_list es') ψ L'.
+    ⊢ have_instruction_type_sem rti sr mr M F L WT WL (to_e_list es') ψ L'.
   Admitted.
 
   Lemma eval_rep_subst_eq ρ ιs s__rep :
@@ -215,15 +218,17 @@ Section Fundamental.
   Proof.
   Admitted.
 
-  Lemma compat_copy M F L wt wt' wl wl' wlf τ es' :
+  Lemma compat_copy M F L wt wt' wtf wl wl' wlf τ es' :
     let fe := fe_of_context F in
+    let WT := wt ++ wt' ++ wtf in
+    let WL := wl ++ wl' ++ wlf in
     let ψ := InstrT [τ] [τ; τ] in
     has_copyability F τ ExCopy ->
     has_instruction_type_ok F ψ L ->
     run_codegen (compile_instr mr fe (ICopy ψ)) wt wl = inr ((), wt', wl', es') ->
-    ⊢ have_instruction_type_sem rti sr mr M F L (wl ++ wl' ++ wlf) (to_e_list es') ψ L.
+    ⊢ have_instruction_type_sem rti sr mr M F L WT WL (to_e_list es') ψ L.
   Proof.
-    intros fe ψ Hcopy Hok Hcompile.
+    intros fe WT WL ψ Hcopy Hok Hcompile.
     unfold compile_instr in Hcompile.
     inv_cg_bind Hcompile ρ wt1 wt1' wl1 wl1' es_nil es1 Htype_rep Hcompile.
     inv_cg_bind Hcompile ιs wt2 wt2' wl2 wl2' es_nil' es2 Heval_rep Hcompile.
@@ -273,31 +278,37 @@ Section Fundamental.
     *)
   Admitted.
 
-  Lemma compat_drop M F L wt wt' wl wl' wlf τ es' :
+  Lemma compat_drop M F L wt wt' wtf wl wl' wlf τ es' :
     let fe := fe_of_context F in
+    let WT := wt ++ wt' ++ wtf in
+    let WL := wl ++ wl' ++ wlf in
     let ψ := InstrT [τ] [] in
     has_dropability F τ ExDrop ->
     has_instruction_type_ok F ψ L ->
     run_codegen (compile_instr mr fe (IDrop ψ)) wt wl = inr ((), wt', wl', es') ->
-    ⊢ have_instruction_type_sem rti sr mr M F L (wl ++ wl' ++ wlf) (to_e_list es') ψ L.
+    ⊢ have_instruction_type_sem rti sr mr M F L WT WL (to_e_list es') ψ L.
   Admitted.
 
-  Lemma compat_num M F L wt wt' wl wl' wlf ψ e es' :
+  Lemma compat_num M F L wt wt' wtf wl wl' wlf ψ e es' :
     let fe := fe_of_context F in
+    let WT := wt ++ wt' ++ wtf in
+    let WL := wl ++ wl' ++ wlf in
     has_instruction_type_num e ψ ->
     has_instruction_type_ok F ψ L ->
     run_codegen (compile_instr mr fe (INum ψ e)) wt wl = inr ((), wt', wl', es') ->
-    ⊢ have_instruction_type_sem rti sr mr M F L (wl ++ wl' ++ wlf) (to_e_list es') ψ L.
+    ⊢ have_instruction_type_sem rti sr mr M F L WT WL (to_e_list es') ψ L.
   Admitted.
 
-  Lemma compat_num_const M F L wt wt' wl wl' wlf n ν es' :
+  Lemma compat_num_const M F L wt wt' wtf wl wl' wlf n ν es' :
     let fe := fe_of_context F in
+    let WT := wt ++ wt' ++ wtf in
+    let WL := wl ++ wl' ++ wlf in
     let ψ := InstrT [] [num_type_type ν] in
     has_instruction_type_ok F ψ L ->
     run_codegen (compile_instr mr fe (INumConst ψ n)) wt wl = inr ((), wt', wl', es') ->
-    ⊢ have_instruction_type_sem rti sr mr M F L (wl ++ wl' ++ wlf) (to_e_list es') ψ L.
+    ⊢ have_instruction_type_sem rti sr mr M F L WT WL (to_e_list es') ψ L.
   Proof.
-    intros fe ψ Hok Hcompile. cbn in Hcompile.
+    intros fe WT WL ψ Hok Hcompile. cbn in Hcompile.
     (* Immediately, we must destruct ν *)
     destruct ν; cbn in Hcompile; inversion Hcompile.
     (* From here on out, we have an integer case and a float case (until we split
@@ -653,7 +664,7 @@ Section Fundamental.
       erewrite IHvh;eauto. 
     }
   Qed.
-  
+
   Lemma lh_depth_pull_base_l_take_len {i : nat} (vh : valid_holed i) (len : nat) vh' vs :
     pull_base_l_drop_len vh len = (vh', vs) ->
     lh_depth (lh_of_vh vh) = lh_depth (lh_of_vh vh').
@@ -738,19 +749,23 @@ Section Fundamental.
     }
   Qed. *)
 
-  Lemma compat_block M F L L' wt wt' wl wl' wlf τs1 τs2 es es' :
+  Lemma compat_block M F L L' wt wt' wtf wl wl' wlf τs1 τs2 es es' :
     let fe := fe_of_context F in
+    let WT := wt ++ wt' ++ wtf in
+    let WL := wl ++ wl' ++ wlf in
     let F' := F <| fc_labels ::= cons (τs2, L') |> in
     let ψ := InstrT τs1 τs2 in
     has_instruction_type_ok F ψ L' ->
-    (forall wt wt' wl wl' wlf es',
+    (forall wt wt' wtf wl wl' wlf es',
         let fe' := fe_of_context F' in
+        let WT := wt ++ wt' ++ wtf in
+        let WL := wl ++ wl' ++ wlf in
         run_codegen (compile_instrs mr fe' es) wt wl = inr ((), wt', wl', es') ->
-        ⊢ have_instruction_type_sem rti sr mr M F' L (wl ++ wl' ++ wlf) (to_e_list es') ψ L') ->
+        ⊢ have_instruction_type_sem rti sr mr M F' L WT WL (to_e_list es') ψ L') ->
     run_codegen (compile_instr mr fe (IBlock ψ L' es)) wt wl = inr ((), wt', wl', es') ->
-    ⊢ have_instruction_type_sem rti sr mr M F L (wl ++ wl' ++ wlf) (to_e_list es') ψ L'.
+    ⊢ have_instruction_type_sem rti sr mr M F L WT WL (to_e_list es') ψ L'.
   Proof.
-    intros fe F' ψ Hok IH Hrun.
+    intros fe F' WT WL ψ Hok IH Hrun.
     cbn [compile_instr] in Hrun.
     inv_cg_bind Hrun ρ wt0 wt0' wl0 wl0' es_nil es0' Hrun1 Hrun2.
     subst wt' wl' es'.
@@ -770,7 +785,6 @@ Section Fundamental.
     clear Hretval.
     apply run_codegen_capture in Hrun1 as [Hrun1 ->].
     eapply IH in Hrun1.
-    rewrite app_nil_r app_nil_l. 
     unfold have_instruction_type_sem.
     iSimpl.
     (*
@@ -1030,36 +1044,46 @@ Section Fundamental.
     *)
   Admitted. 
 
-  Lemma compat_loop M F L wt wt' wl wl' wlf es es' τs1 τs2 :
+  Lemma compat_loop M F L wt wt' wtf wl wl' wlf es es' τs1 τs2 :
     let fe := fe_of_context F in
+    let WT := wt ++ wt' ++ wtf in
+    let WL := wl ++ wl' ++ wlf in
     let F' := F <| fc_labels ::= cons (τs1, L) |> in
     let ψ := InstrT τs1 τs2 in
     has_instruction_type_ok F ψ L ->
-    (forall wt wt' wl wl' wlf es',
+    (forall wt wt' wtf wl wl' wlf es',
         let fe' := fe_of_context F' in
+        let WT := wt ++ wt' ++ wtf in
+        let WL := wl ++ wl' ++ wlf in
         run_codegen (compile_instrs mr fe' es) wt wl = inr ((), wt', wl', es') ->
-        ⊢ have_instruction_type_sem rti sr mr M F' L (wl ++ wl' ++ wlf) (to_e_list es') ψ L) ->
+        ⊢ have_instruction_type_sem rti sr mr M F' L WT WL (to_e_list es') ψ L) ->
     run_codegen (compile_instr mr fe (ILoop ψ es)) wt wl = inr ((), wt', wl', es') ->
-    ⊢ have_instruction_type_sem rti sr mr M F L (wl ++ wl' ++ wlf) (to_e_list es') ψ L.
+    ⊢ have_instruction_type_sem rti sr mr M F L WT WL (to_e_list es') ψ L.
   Admitted.
 
-  Lemma compat_ite M F L L' wt wt' wl wl' wlf es1 es2 es' τs1 τs2 :
+  Lemma compat_ite M F L L' wt wt' wtf wl wl' wlf es1 es2 es' τs1 τs2 :
     let fe := fe_of_context F in
+    let WT := wt ++ wt' ++ wtf in
+    let WL := wl ++ wl' ++ wlf in
     let F' := F <| fc_labels ::= cons (τs2, L') |> in
     let ψ := InstrT (τs1 ++ [type_i32]) τs2 in
     has_instruction_type_ok F ψ L' ->
-    (forall wt wt' wl wl' wlf es',
+    (forall wt wt' wtf wl wl' wlf es',
         let fe := fe_of_context F' in
+        let WT := wt ++ wt' ++ wtf in
+        let WL := wl ++ wl' ++ wlf in
         run_codegen (compile_instrs mr fe es1) wt wl = inr ((), wt', wl', es') ->
-        ⊢ have_instruction_type_sem rti sr mr M F' L (wl ++ wl' ++ wlf) (to_e_list es') (InstrT τs1 τs2) L') ->
-    (forall wt wt' wl wl' wlf es',
+        ⊢ have_instruction_type_sem rti sr mr M F' L WT WL (to_e_list es') (InstrT τs1 τs2) L') ->
+    (forall wt wt' wtf wl wl' wlf es',
         let fe := fe_of_context F' in
+        let WT := wt ++ wt' ++ wtf in
+        let WL := wl ++ wl' ++ wlf in
         run_codegen (compile_instrs mr fe es2) wt wl = inr ((), wt', wl', es') ->
-        ⊢ have_instruction_type_sem rti sr mr M F' L (wl ++ wl' ++ wlf) (to_e_list es') (InstrT τs1 τs2) L') ->
+        ⊢ have_instruction_type_sem rti sr mr M F' L WT WL (to_e_list es') (InstrT τs1 τs2) L') ->
     run_codegen (compile_instr mr fe (IIte ψ L' es1 es2)) wt wl = inr ((), wt', wl', es') ->
-    ⊢ have_instruction_type_sem rti sr mr M F L (wl ++ wl' ++ wlf) (to_e_list es') ψ L'.
+    ⊢ have_instruction_type_sem rti sr mr M F L WT WL (to_e_list es') ψ L'.
   Proof.
-    intros fe F' ψ Hok Hthen Helse Hcodegen.
+    intros fe WT WL F' ψ Hok Hthen Helse Hcodegen.
     iIntros (smem srep ssize se inst fr lh rvs vs) "%Hsubst #Hinst #Hctxt Hrvs Hvss Hvsl Hfr Hrun".
     iDestruct "Hvss" as (vss) "(-> & Hvss)".
     (*
@@ -1532,78 +1556,91 @@ Section Fundamental.
     *)
   Admitted.
 
-  Lemma compat_br M F L L' wt wt' wl wl' wlf es' i τs1 τs τs2 :
+  Lemma compat_br M F L L' wt wt' wtf wl wl' wlf es' i τs1 τs τs2 :
     let fe := fe_of_context F in
+    let WT := wt ++ wt' ++ wtf in
+    let WL := wl ++ wl' ++ wlf in
     let ψ := InstrT (τs1 ++ τs) τs2 in
     F.(fc_labels) !! i = Some (τs, L) ->
     Forall (fun τ => has_dropability F τ ImDrop) τs1 ->
     has_instruction_type_ok F ψ L' ->
     run_codegen (compile_instr mr fe (IBr ψ i)) wt wl = inr ((), wt', wl', es') ->
-    ⊢ have_instruction_type_sem rti sr mr M F L (wl ++ wl' ++ wlf) (to_e_list es') ψ L'.
+    ⊢ have_instruction_type_sem rti sr mr M F L WT WL (to_e_list es') ψ L'.
   Admitted.
 
-  Lemma compat_return M F L L' wt wt' wl wl' wlf es' τs1 τs τs2 :
+  Lemma compat_return M F L L' wt wt' wtf wl wl' wlf es' τs1 τs τs2 :
     let fe := fe_of_context F in
+    let WT := wt ++ wt' ++ wtf in
+    let WL := wl ++ wl' ++ wlf in
     let ψ := InstrT (τs1 ++ τs) τs2 in
     F.(fc_return) = τs ->
     Forall (fun τ => has_dropability F τ ImDrop) τs1 ->
     has_instruction_type_ok F ψ L' ->
     run_codegen (compile_instr mr fe (IReturn ψ)) wt wl = inr ((), wt', wl', es') ->
-    ⊢ have_instruction_type_sem rti sr mr M F L (wl ++ wl' ++ wlf) (to_e_list es') ψ L'.
+    ⊢ have_instruction_type_sem rti sr mr M F L WT WL (to_e_list es') ψ L'.
   Admitted.
 
-  Lemma compat_local_get_copy M F L wt wt' wl wl' wlf es' i τ :
+  Lemma compat_local_get_copy M F L wt wt' wtf wl wl' wlf es' i τ :
     let fe := fe_of_context F in
+    let WT := wt ++ wt' ++ wtf in
+    let WL := wl ++ wl' ++ wlf in
     let ψ := InstrT [] [τ] in
     L !! i = Some (Some τ) ->
     has_copyability F τ ImCopy ->
     has_instruction_type_ok F ψ L ->
     run_codegen (compile_instr mr fe (ILocalGet ψ i)) wt wl = inr ((), wt', wl', es') ->
-    ⊢ have_instruction_type_sem rti sr mr M F L (wl ++ wl' ++ wlf) (to_e_list es') ψ L.
+    ⊢ have_instruction_type_sem rti sr mr M F L WT WL (to_e_list es') ψ L.
   Admitted.
 
-  Lemma compat_local_get_move M F L wt wt' wl wl' wlf es' i τ :
+  Lemma compat_local_get_move M F L wt wt' wtf wl wl' wlf es' i τ :
     let fe := fe_of_context F in
+    let WT := wt ++ wt' ++ wtf in
+    let WL := wl ++ wl' ++ wlf in
     let ψ := InstrT [] [τ] in
     let L' := <[ i := None]> L in
     L !! i = Some (Some τ) ->
     has_instruction_type_ok F ψ L' ->
     run_codegen (compile_instr mr fe (ILocalGet ψ i)) wt wl = inr ((), wt', wl', es') ->
-    ⊢ have_instruction_type_sem rti sr mr M F L (wl ++ wl' ++ wlf) (to_e_list es') ψ L'.
+    ⊢ have_instruction_type_sem rti sr mr M F L WT WL (to_e_list es') ψ L'.
   Admitted.
 
-  Lemma compat_local_set M F L wt wt' wl wl' wlf es' i τ :
+  Lemma compat_local_set M F L wt wt' wtf wl wl' wlf es' i τ :
     let fe := fe_of_context F in
+    let WT := wt ++ wt' ++ wtf in
+    let WL := wl ++ wl' ++ wlf in
     let ψ := InstrT [τ] [] in
     let L' := <[ i := Some τ ]> L in
     (∀ τ0, L !! i = Some (Some τ0) → has_dropability F τ0 ImDrop) ->
     has_instruction_type_ok F ψ L' ->
     run_codegen (compile_instr mr fe (ILocalSet ψ i)) wt wl = inr ((), wt', wl', es') ->
-    ⊢ have_instruction_type_sem rti sr mr M F L (wl ++ wl' ++ wlf) (to_e_list es') ψ L'.
+    ⊢ have_instruction_type_sem rti sr mr M F L WT WL (to_e_list es') ψ L'.
   Admitted.
 
-  Lemma compat_coderef M F L wt wt' wl wl' wlf es' i ϕ :
+  Lemma compat_coderef M F L wt wt' wtf wl wl' wlf es' i ϕ :
     let fe := fe_of_context F in
+    let WT := wt ++ wt' ++ wtf in
+    let WL := wl ++ wl' ++ wlf in
     let τ := CodeRefT (VALTYPE (PrimR I32R) ImCopy ImDrop) ϕ in
     let ψ := InstrT [] [τ] in
     M.(mc_table) !! i = Some ϕ ->
     has_instruction_type_ok F ψ L ->
     run_codegen (compile_instr mr fe (ICodeRef ψ i)) wt wl = inr ((), wt', wl', es') ->
-    ⊢ have_instruction_type_sem rti sr mr M F L (wl ++ wl' ++ wlf) (to_e_list es') ψ L.
+    ⊢ have_instruction_type_sem rti sr mr M F L WT WL (to_e_list es') ψ L.
   Admitted.
 
-  Lemma compat_inst M F L wt wt' wl wl' wlf es' ix ϕ ϕ' :
+  Lemma compat_inst M F L wt wt' wtf wl wl' wlf es' ix ϕ ϕ' :
     let fe := fe_of_context F in
+    let WT := wt ++ wt' ++ wtf in
+    let WL := wl ++ wl' ++ wlf in
     let κ := VALTYPE (PrimR I32R) ImCopy ImDrop in
     let ψ := InstrT [CodeRefT κ ϕ] [CodeRefT κ ϕ'] in
     function_type_inst F ix ϕ ϕ' ->
     has_instruction_type_ok F ψ L ->
     run_codegen (compile_instr mr fe (IInst ψ ix)) wt wl = inr ((), wt', wl', es') ->
-    ⊢ have_instruction_type_sem rti sr mr M F L (wl ++ wl' ++ wlf) (to_e_list es') ψ L.
+    ⊢ have_instruction_type_sem rti sr mr M F L WT WL (to_e_list es') ψ L.
   Proof.
-    intros fe κ ψ Hfinst Hok Hcg.
-    cbn in Hcg; inversion Hcg; subst wl' es'; clear Hcg.
-    rewrite app_nil_l.
+    intros fe WT WL κ ψ Hfinst Hok Hcg.
+    cbn in Hcg; inversion Hcg; subst wt' wl' es'; clear Hcg.
     simpl to_e_list.
     iApply sem_type_erased; first done.
     iIntros (se s__mem s__rep s__size vs) "Hrec".
@@ -1626,95 +1663,113 @@ Section Fundamental.
     admit.
   Admitted.
 
-  Lemma compat_call M F L wt wt' wl wl' wlf es' i ixs ϕ τs1 τs2 :
+  Lemma compat_call M F L wt wt' wtf wl wl' wlf es' i ixs ϕ τs1 τs2 :
     let fe := fe_of_context F in
+    let WT := wt ++ wt' ++ wtf in
+    let WL := wl ++ wl' ++ wlf in
     let ψ := InstrT τs1 τs2 in
     M.(mc_functions) !! i = Some ϕ ->
     function_type_insts F ixs ϕ (MonoFunT τs1 τs2) ->
     has_instruction_type_ok F ψ L ->
     run_codegen (compile_instr mr fe (ICall ψ i ixs)) wt wl = inr ((), wt', wl', es') ->
-    ⊢ have_instruction_type_sem rti sr mr M F L (wl ++ wl' ++ wlf) (to_e_list es') ψ L.
+    ⊢ have_instruction_type_sem rti sr mr M F L WT WL (to_e_list es') ψ L.
   Admitted.
 
-  Lemma compat_call_indirect M F L wt wt' wl wl' wlf es' τs1 τs2 :
+  Lemma compat_call_indirect M F L wt wt' wtf wl wl' wlf es' τs1 τs2 :
     let fe := fe_of_context F in
+    let WT := wt ++ wt' ++ wtf in
+    let WL := wl ++ wl' ++ wlf in
     let κ := VALTYPE (PrimR I32R) ImCopy ImDrop in
     let ψ := InstrT (τs1 ++ [CodeRefT κ (MonoFunT τs1 τs2)]) τs2 in
     has_instruction_type_ok F ψ L ->
     run_codegen (compile_instr mr fe (ICallIndirect ψ)) wt wl = inr ((), wt', wl', es') ->
-    ⊢ have_instruction_type_sem rti sr mr M F L (wl ++ wl' ++ wlf) (to_e_list es') ψ L.
+    ⊢ have_instruction_type_sem rti sr mr M F L WT WL (to_e_list es') ψ L.
   Admitted.
 
-  Lemma compat_inject_sum M F L wt wt' wl wl' wlf es' i τs τ κ :
+  Lemma compat_inject_sum M F L wt wt' wtf wl wl' wlf es' i τs τ κ :
     let fe := fe_of_context F in
+    let WT := wt ++ wt' ++ wtf in
+    let WL := wl ++ wl' ++ wlf in
     let ψ := InstrT [τ] [SumT κ τs] in
     τs !! i = Some τ ->
     has_instruction_type_ok F ψ L ->
     run_codegen (compile_instr mr fe (IInject ψ i)) wt wl = inr ((), wt', wl', es') ->
-    ⊢ have_instruction_type_sem rti sr mr M F L (wl ++ wl' ++ wlf) (to_e_list es') ψ L.
+    ⊢ have_instruction_type_sem rti sr mr M F L WT WL (to_e_list es') ψ L.
   Admitted.
 
-  Lemma compat_inject_variant M F L wt wt' wl wl' wlf es' μ i τ τs κr κv κs :
+  Lemma compat_inject_variant M F L wt wt' wtf wl wl' wlf es' μ i τ τs κr κv κs :
     let fe := fe_of_context F in
+    let WT := wt ++ wt' ++ wtf in
+    let WL := wl ++ wl' ++ wlf in
     let τs' := zip_with SerT κs τs in
     let ψ := InstrT [τ] [RefT κr μ (VariantT κv τs)] in
     τs !! i = Some τ ->
     mono_mem μ ->
     has_instruction_type_ok F ψ L ->
     run_codegen (compile_instr mr fe (IInject ψ i)) wt wl = inr ((), wt', wl', es') ->
-    ⊢ have_instruction_type_sem rti sr mr M F L (wl ++ wl' ++ wlf) (to_e_list es') ψ L.
+    ⊢ have_instruction_type_sem rti sr mr M F L WT WL (to_e_list es') ψ L.
   Admitted.
 
-  Lemma compat_case_sum M F L L' wt wt' wl wl' wlf es' ess τ' τs κ :
+  Lemma compat_case_sum M F L L' wt wt' wtf wl wl' wlf es' ess τ' τs κ :
     let fe := fe_of_context F in
+    let WT := wt ++ wt' ++ wtf in
+    let WL := wl ++ wl' ++ wlf in
     let ψ := InstrT [SumT κ τs] [τ'] in
     Forall2
       (fun τ es =>
-         forall wt wt' wl wl' wlf es',
+         forall wt wt' wtf wl wl' wlf es',
+           let WT := wt ++ wt' ++ wtf in
+           let WL := wl ++ wl' ++ wlf in
            run_codegen (compile_instrs mr fe es) wt wl = inr ((), wt', wl', es') ->
-           ⊢ have_instruction_type_sem rti sr mr M F L (wl ++ wl' ++ wlf) (to_e_list es') (InstrT [τ] [τ']) L')
+           ⊢ have_instruction_type_sem rti sr mr M F L WT WL (to_e_list es') (InstrT [τ] [τ']) L')
       τs ess ->
     has_instruction_type_ok F ψ L' ->
     run_codegen (compile_instr mr fe (ICase ψ L' ess)) wt wl = inr ((), wt', wl', es') ->
-    ⊢ have_instruction_type_sem rti sr mr M F L (wl ++ wl' ++ wlf) (to_e_list es') ψ L'.
+    ⊢ have_instruction_type_sem rti sr mr M F L WT WL (to_e_list es') ψ L'.
   Admitted.
 
-  Lemma compat_case_variant M F L L' wt wt' wl wl' wlf ess es' τ' τs μ κr κv κs :
+  Lemma compat_case_variant M F L L' wt wt' wtf wl wl' wlf ess es' τ' τs μ κr κv κs :
     let fe := fe_of_context F in
+    let WT := wt ++ wt' ++ wtf in
+    let WL := wl ++ wl' ++ wlf in
     let τs' := zip_with SerT κs τs in
     let ψ := InstrT [RefT κr μ (VariantT κv τs')] [τ'] in
     Forall2
       (fun τ es =>
-         forall wt wt' wl wl' wlf es',
+         forall wt wt' wtf wl wl' wlf es',
+           let WT := wt ++ wt' ++ wtf in
+           let WL := wl ++ wl' ++ wlf in
            run_codegen (compile_instrs mr fe es) wt wl = inr ((), wt', wl', es') ->
-           ⊢ have_instruction_type_sem rti sr mr M F L (wl ++ wl' ++ wlf)
-               (to_e_list es') (InstrT [τ] [τ']) L')
+           ⊢ have_instruction_type_sem rti sr mr M F L WT WL (to_e_list es') (InstrT [τ] [τ']) L')
       τs' ess ->
     has_instruction_type_ok F ψ L' ->
     run_codegen (compile_instr mr fe (ICase ψ L' ess)) wt wl = inr ((), wt', wl', es') ->
-    ⊢ have_instruction_type_sem rti sr mr M F L (wl ++ wl' ++ wlf) (to_e_list es') ψ L'.
+    ⊢ have_instruction_type_sem rti sr mr M F L WT WL (to_e_list es') ψ L'.
   Admitted.
 
-  Lemma compat_group M F L wt wt' wl wl' wlf es' τs κ :
+  Lemma compat_group M F L wt wt' wtf wl wl' wlf es' τs κ :
     let fe := fe_of_context F in
+    let WT := wt ++ wt' ++ wtf in
+    let WL := wl ++ wl' ++ wlf in
     let ψ := InstrT τs [ProdT κ τs] in
     has_instruction_type_ok F ψ L ->
     run_codegen (compile_instr mr fe (IGroup ψ)) wt wl = inr ((), wt', wl', es') ->
-    ⊢ have_instruction_type_sem rti sr mr M F L (wl ++ wl' ++ wlf) (to_e_list es') ψ L.
+    ⊢ have_instruction_type_sem rti sr mr M F L WT WL (to_e_list es') ψ L.
   Admitted.
 
-  Lemma compat_ungroup M F L wt wt' wl wl' wlf es' τs κ :
+  Lemma compat_ungroup M F L wt wt' wtf wl wl' wlf es' τs κ :
     let fe := fe_of_context F in
+    let WT := wt ++ wt' ++ wtf in
+    let WL := wl ++ wl' ++ wlf in
     let ψ := InstrT [ProdT κ τs] τs in
     has_instruction_type_ok F ψ L ->
     run_codegen (compile_instr mr fe (IUngroup ψ)) wt wl = inr ((), wt', wl', es') ->
-    ⊢ have_instruction_type_sem rti sr mr M F L (wl ++ wl' ++ wlf) (to_e_list es') ψ L.
+    ⊢ have_instruction_type_sem rti sr mr M F L WT WL (to_e_list es') ψ L.
   Proof.
-    intros fe ψ Hok Hcg.
+    intros fe WT WL ψ Hok Hcg.
     inversion Hok as [F' ψ' L' Hmono Hok'].
     subst F' ψ' L'.
     cbn in Hcg; inversion Hcg; subst wt' wl' es'.
-    rewrite app_nil_l.
     simpl to_e_list.
     iApply sem_type_erased_nop; first done.
     iIntros (se s__mem s__rep s__size vs) "Hvs".
@@ -1739,17 +1794,18 @@ Section Fundamental.
     by rewrite big_sepL2_flip.
   Qed.
 
-  Lemma compat_fold M F L wt wt' wl wl' wlf es' τ κ :
+  Lemma compat_fold M F L wt wt' wtf wl wl' wlf es' τ κ :
     let fe := fe_of_context F in
+    let WT := wt ++ wt' ++ wtf in
+    let WL := wl ++ wl' ++ wlf in
     let τ0 := subst_type VarM VarR VarS (unscoped.scons (RecT κ τ) VarT) τ in
     let ψ := InstrT [τ0] [RecT κ τ] in
     has_instruction_type_ok F ψ L ->
     run_codegen (compile_instr mr fe (IFold ψ)) wt wl = inr ((), wt', wl', es') ->
-    ⊢ have_instruction_type_sem rti sr mr M F L (wl ++ wl' ++ wlf) (to_e_list es') ψ L.
+    ⊢ have_instruction_type_sem rti sr mr M F L WT WL (to_e_list es') ψ L.
   Proof.
-    intros fe τrec ψ Hok Hcg.
-    cbn in Hcg; inversion Hcg; subst wl' es'; clear Hcg.
-    rewrite app_nil_l.
+    intros fe WT WL τrec ψ Hok Hcg.
+    cbn in Hcg; inversion Hcg; subst wt' wl' es'; clear Hcg.
     simpl to_e_list.
     iApply sem_type_erased; first done.
     iIntros (se s__mem s__rep s__size vs) "Hrec".
@@ -1758,17 +1814,18 @@ Section Fundamental.
     admit.
   Admitted.
 
-  Lemma compat_unfold M F L wt wt' wl wl' wlf es' τ κ :
+  Lemma compat_unfold M F L wt wt' wtf wl wl' wlf es' τ κ :
     let fe := fe_of_context F in
+    let WT := wt ++ wt' ++ wtf in
+    let WL := wl ++ wl' ++ wlf in
     let τ0 := subst_type VarM VarR VarS (unscoped.scons (RecT κ τ) VarT) τ in
     let ψ := InstrT [RecT κ τ] [τ0] in
     has_instruction_type_ok F ψ L ->
     run_codegen (compile_instr mr fe (IUnfold ψ)) wt wl = inr ((), wt', wl', es') ->
-    ⊢ have_instruction_type_sem rti sr mr M F L (wl ++ wl' ++ wlf) (to_e_list es') ψ L.
+    ⊢ have_instruction_type_sem rti sr mr M F L WT WL (to_e_list es') ψ L.
   Proof.
-    intros fe τrec ψ Hok Hcg.
-    cbn in Hcg; inversion Hcg; subst wl' es'; clear Hcg.
-    rewrite app_nil_l.
+    intros fe WT WL τrec ψ Hok Hcg.
+    cbn in Hcg; inversion Hcg; subst wt' wl' es'; clear Hcg.
     simpl to_e_list.
     iApply sem_type_erased; first done.
     iIntros (se s__mem s__rep s__size vs) "Hrec".
@@ -1777,35 +1834,40 @@ Section Fundamental.
     admit.
   Admitted.
 
-  Lemma compat_pack M F L wt wt' wl wl' wlf es' τ τ' :
+  Lemma compat_pack M F L wt wt' wtf wl wl' wlf es' τ τ' :
     let fe := fe_of_context F in
+    let WT := wt ++ wt' ++ wtf in
+    let WL := wl ++ wl' ++ wlf in
     let ψ := InstrT [τ] [τ'] in
     packed_existential F τ τ' ->
     has_instruction_type_ok F ψ L ->
     run_codegen (compile_instr mr fe (IPack ψ)) wt wl = inr ((), wt', wl', es') ->
-    ⊢ have_instruction_type_sem rti sr mr M F L (wl ++ wl' ++ wlf) (to_e_list es') ψ L.
+    ⊢ have_instruction_type_sem rti sr mr M F L WT WL (to_e_list es') ψ L.
   Proof.
-    intros fe τrec ψ Hok Hcg.
-    cbn in Hcg; inversion Hcg; subst wl' es'; clear Hcg.
-    rewrite app_nil_l.
+    intros fe WT WL τrec ψ Hok Hcg.
+    cbn in Hcg; inversion Hcg; subst wt' wl' es'; clear Hcg.
     simpl to_e_list.
     iApply sem_type_erased; first done.
     iIntros (se s__mem s__rep s__size vs) "Hrec".
     do 2 rewrite values_interp_one_eq value_interp_eq.
   Admitted.
 
-  Lemma compat_unpack M F F0' L L' L0 L0' wt wt' wl wl' wlf es es' es0 τs1 τs2 ψ0 :
+  Lemma compat_unpack M F F0' L L' L0 L0' wt wt' wtf wl wl' wlf es es' es0 τs1 τs2 ψ0 :
     let fe := fe_of_context F in
+    let WT := wt ++ wt' ++ wtf in
+    let WL := wl ++ wl' ++ wlf in
     let F' := F <| fc_labels ::= cons (τs2, L') |> in
     let ψ := InstrT τs1 τs2 in
     unpacked_existential F' L es ψ L' F0' L0 es0 ψ0 L0' ->
     has_instruction_type_ok F ψ L' ->
-    (forall wt wt' wl wl' wlf es',
+    (forall wt wt' wtf wl wl' wlf es',
         let fe0' := fe_of_context F0' in
+        let WT := wt ++ wt' ++ wtf in
+        let WL := wl ++ wl' ++ wlf in
         run_codegen (compile_instrs mr fe0' es0) wt wl = inr ((), wt', wl', es') ->
-        ⊢ have_instruction_type_sem rti sr mr M F0' L0 (wl ++ wl' ++ wlf) (to_e_list es') ψ0 L0') ->
+        ⊢ have_instruction_type_sem rti sr mr M F0' L0 WT WL (to_e_list es') ψ0 L0') ->
     run_codegen (compile_instr mr fe (IUnpack ψ L' es)) wt wl = inr ((), wt', wl', es') ->
-    ⊢ have_instruction_type_sem rti sr mr M F L (wl ++ wl' ++ wlf) (to_e_list es') ψ L'.
+    ⊢ have_instruction_type_sem rti sr mr M F L WT WL (to_e_list es') ψ L'.
   Admitted.
 
   Lemma length1concat (vss: list (list value)) (vs: list value):
@@ -1819,14 +1881,16 @@ Section Fundamental.
     by rewrite app_nil_r.
   Qed.
 
-  Lemma compat_tag M F L wt wt' wl wl' wlf es' :
+  Lemma compat_tag M F L wt wt' wtf wl wl' wlf es' :
     let fe := fe_of_context F in
+    let WT := wt ++ wt' ++ wtf in
+    let WL := wl ++ wl' ++ wlf in
     let ψ := InstrT [type_i32] [type_i31] in
     has_instruction_type_ok F ψ L ->
     run_codegen (compile_instr mr fe (ITag ψ)) wt wl = inr ((), wt', wl', es') ->
-    ⊢ have_instruction_type_sem rti sr mr M F L (wl ++ wl' ++ wlf) (to_e_list es') ψ L.
+    ⊢ have_instruction_type_sem rti sr mr M F L WT WL (to_e_list es') ψ L.
   Proof.
-    intros fe ψ Hok Hcompile.
+    intros fe WT WL ψ Hok Hcompile.
     cbn in Hcompile; inversion Hcompile; subst; clear Hcompile.
 
     iIntros (? ? ? ? ? ? ? ? ?) "%Henv #Hinst #Hlf Hrvs Hvs Hframe Hfr Hrun".
@@ -1908,14 +1972,16 @@ Section Fundamental.
         by unfold primitive_rep_interp.
   Qed.
 
-  Lemma compat_untag M F L wt wt' wl wl' wlf es' :
+  Lemma compat_untag M F L wt wt' wtf wl wl' wlf es' :
     let fe := fe_of_context F in
+    let WT := wt ++ wt' ++ wtf in
+    let WL := wl ++ wl' ++ wlf in
     let ψ := InstrT [type_i31] [type_i32] in
     has_instruction_type_ok F ψ L ->
     run_codegen (compile_instr mr fe (IUntag ψ)) wt wl = inr ((), wt', wl', es') ->
-    ⊢ have_instruction_type_sem rti sr mr M F L (wl ++ wl' ++ wlf) (to_e_list es') ψ L.
+    ⊢ have_instruction_type_sem rti sr mr M F L WT WL (to_e_list es') ψ L.
   Proof.
-    intros fe ψ Hok Hcompile.
+    intros fe WT WL ψ Hok Hcompile.
     cbn in Hcompile; inversion Hcompile; subst; clear Hcompile.
 
     iIntros (? ? ? ? ? ? ? ? ?) "%Henv #Hinst #Hlf Hrvs Hvs Hframe Hfr Hrun".
@@ -1992,26 +2058,32 @@ Section Fundamental.
       by unfold primitive_rep_interp.
   Qed.
 
-  Lemma compat_cast M F L wt wt' wl wl' wlf es' τ τ' :
+  Lemma compat_cast M F L wt wt' wtf wl wl' wlf es' τ τ' :
     let fe := fe_of_context F in
+    let WT := wt ++ wt' ++ wtf in
+    let WL := wl ++ wl' ++ wlf in
     let ψ := InstrT [τ] [τ'] in
     type_eq F τ τ' ->
     has_instruction_type_ok F ψ L ->
     run_codegen (compile_instr mr fe (ICast ψ)) wt wl = inr ((), wt', wl', es') ->
-    ⊢ have_instruction_type_sem rti sr mr M F L (wl ++ wl' ++ wlf) (to_e_list es') ψ L.
+    ⊢ have_instruction_type_sem rti sr mr M F L WT WL (to_e_list es') ψ L.
   Admitted.
 
-  Lemma compat_new M F L wt wt' wl wl' wlf κ κser μ τ es' :
+  Lemma compat_new M F L wt wt' wtf wl wl' wlf κ κser μ τ es' :
     let fe := fe_of_context F in
+    let WT := wt ++ wt' ++ wtf in
+    let WL := wl ++ wl' ++ wlf in
     let ψ := InstrT [τ] [RefT κ μ (SerT κser τ)] in
     mono_mem μ ->
     has_instruction_type_ok F ψ L ->
     run_codegen (compile_instr mr fe (INew ψ)) wt wl = inr ((), wt', wl', es') ->
-    ⊢ have_instruction_type_sem rti sr mr M F L (wl ++ wl' ++ wlf) (to_e_list es') ψ L.
+    ⊢ have_instruction_type_sem rti sr mr M F L WT WL (to_e_list es') ψ L.
   Admitted.
 
-  Lemma compat_load_copy M F L wt wt' wl wl' wlf es' κ κser μ τ τval π pr :
+  Lemma compat_load_copy M F L wt wt' wtf wl wl' wlf es' κ κser μ τ τval π pr :
     let fe := fe_of_context F in
+    let WT := wt ++ wt' ++ wtf in
+    let WL := wl ++ wl' ++ wlf in
     let ψ := InstrT [RefT κ μ τ] [RefT κ μ τ; τval] in
     has_copyability F τval ExCopy ->
     resolves_path τ π None pr ->
@@ -2019,11 +2091,13 @@ Section Fundamental.
     Forall (mono_size F) (pr_prefix pr) ->
     has_instruction_type_ok F ψ L ->
     run_codegen (compile_instr mr fe (ILoad ψ π Copy)) wt wl = inr ((), wt', wl', es') ->
-    ⊢ have_instruction_type_sem rti sr mr M F L (wl ++ wl' ++ wlf) (to_e_list es') ψ L.
+    ⊢ have_instruction_type_sem rti sr mr M F L WT WL (to_e_list es') ψ L.
   Admitted.
 
-  Lemma compat_load_move M F L wt wt' wl wl' wlf es' κ κ' κser σ τ τval π pr :
+  Lemma compat_load_move M F L wt wt' wtf wl wl' wlf es' κ κ' κser σ τ τval π pr :
     let fe := fe_of_context F in   
+    let WT := wt ++ wt' ++ wtf in
+    let WL := wl ++ wl' ++ wlf in
     let ψ := InstrT [RefT κ (ConstM MemMM) τ] [RefT κ' (ConstM MemMM) (pr_replaced pr); τval] in
     resolves_path τ π (Some (type_uninit σ)) pr ->
     has_size F pr.(pr_target) σ ->
@@ -2031,11 +2105,13 @@ Section Fundamental.
     Forall (mono_size F) (pr_prefix pr) ->
     has_instruction_type_ok F ψ L ->
     run_codegen (compile_instr mr fe (ILoad ψ π Move)) wt wl = inr ((), wt', wl', es') ->
-    ⊢ have_instruction_type_sem rti sr mr M F L (wl ++ wl' ++ wlf) (to_e_list es') ψ L.
+    ⊢ have_instruction_type_sem rti sr mr M F L WT WL (to_e_list es') ψ L.
   Admitted.
 
-  Lemma compat_store_weak M F L wt wt' wl wl' wlf es' κ κser μ τ τval π pr :
+  Lemma compat_store_weak M F L wt wt' wtf wl wl' wlf es' κ κser μ τ τval π pr :
     let fe := fe_of_context F in
+    let WT := wt ++ wt' ++ wtf in
+    let WL := wl ++ wl' ++ wlf in
     let ψ := InstrT [RefT κ μ τ; τval] [RefT κ μ τ] in
     resolves_path τ π None pr ->
     has_dropability F pr.(pr_target) ImDrop ->
@@ -2043,11 +2119,13 @@ Section Fundamental.
     Forall (mono_size F) (pr_prefix pr) ->
     has_instruction_type_ok F ψ L ->
     run_codegen (compile_instr mr fe (IStore ψ π)) wt wl = inr ((), wt', wl', es') ->
-    ⊢ have_instruction_type_sem rti sr mr M F L (wl ++ wl' ++ wlf) (to_e_list es') ψ L.
+    ⊢ have_instruction_type_sem rti sr mr M F L WT WL (to_e_list es') ψ L.
   Admitted.
 
-  Lemma compat_store_strong M F L wt wt' wl wl' wlf es' κ κ' κser σ ρ τ τval π pr :
-    let fe := fe_of_context F in   
+  Lemma compat_store_strong M F L wt wt' wtf wl wl' wlf es' κ κ' κser σ ρ τ τval π pr :
+    let fe := fe_of_context F in
+    let WT := wt ++ wt' ++ wtf in
+    let WL := wl ++ wl' ++ wlf in
     let ψ := InstrT [RefT κ (ConstM MemMM) τ; τval] [RefT κ' (ConstM MemMM) (pr_replaced pr)] in
     resolves_path τ π (Some (SerT κser τval)) pr ->
     has_dropability F pr.(pr_target) ImDrop ->
@@ -2057,26 +2135,30 @@ Section Fundamental.
     Forall (mono_size F) (pr_prefix pr) ->
     has_instruction_type_ok F ψ L ->
     run_codegen (compile_instr mr fe (IStore ψ π)) wt wl = inr ((), wt', wl', es') ->
-    ⊢ have_instruction_type_sem rti sr mr M F L (wl ++ wl' ++ wlf) (to_e_list es') ψ L.
+    ⊢ have_instruction_type_sem rti sr mr M F L WT WL (to_e_list es') ψ L.
   Admitted.
 
-  Lemma compat_swap M F L wt wt' wl wl' wlf es' κ κser μ τ τval π pr :
+  Lemma compat_swap M F L wt wt' wtf wl wl' wlf es' κ κser μ τ τval π pr :
      let fe := fe_of_context F in   
+     let WT := wt ++ wt' ++ wtf in
+     let WL := wl ++ wl' ++ wlf in
      let ψ := InstrT [RefT κ μ τ; τval] [RefT κ μ τ; τval] in
      resolves_path τ π None pr ->
      Forall (mono_size F) (pr_prefix pr) ->
      pr.(pr_target) = SerT κser τval ->
      has_instruction_type_ok F ψ L ->
      run_codegen (compile_instr mr fe (ISwap ψ π)) wt wl = inr ((), wt', wl', es') ->
-     ⊢ have_instruction_type_sem rti sr mr M F L (wl ++ wl' ++ wlf) (to_e_list es') ψ L.
+     ⊢ have_instruction_type_sem rti sr mr M F L WT WL (to_e_list es') ψ L.
   Admitted.
 
-  Lemma compat_nil M F L wt wt' wl wl' wlf es' :
+  Lemma compat_nil M F L wt wt' wtf wl wl' wlf es' :
     let fe := fe_of_context F in
+    let WT := wt ++ wt' ++ wtf in
+    let WL := wl ++ wl' ++ wlf in
     run_codegen (compile_instrs mr fe []) wt wl = inr ((), wt', wl', es') ->
-    ⊢ have_instruction_type_sem rti sr mr M F L (wl ++ wl' ++ wlf) (to_e_list es') (InstrT [] []) L.
+    ⊢ have_instruction_type_sem rti sr mr M F L WT WL (to_e_list es') (InstrT [] []) L.
   Proof.
-    intros fe Hcompile.
+    intros fe WT WL Hcompile.
     cbn in Hcompile.
     inversion Hcompile.
 
@@ -2094,7 +2176,6 @@ Section Fundamental.
     rewrite !app_nil_l.
     unfold expr_interp.
 
-
     iApply lenient_wp_nil.
     unfold lp_combine, denote_logpred; cbn.
     iFrame.
@@ -2109,18 +2190,24 @@ Section Fundamental.
     unfold to_e_list. rewrite mathcomp.ssreflect.seq.map_cat. done.
   Qed.
 
-  Lemma compat_app M F L1 L2 L3 wt wt' wl wl' wlf es' es1 es2 τs1 τs2 τs3 :
+  Lemma compat_app M F L1 L2 L3 wt wt' wtf wl wl' wlf es' es1 es2 τs1 τs2 τs3 :
     let fe := fe_of_context F in
-    (forall wt wt' wl wl' wlf es',
+    let WT := wt ++ wt' ++ wtf in
+    let WL := wl ++ wl' ++ wlf in
+    (forall wt wt' wtf wl wl' wlf es',
+        let WT := wt ++ wt' ++ wtf in
+        let WL := wl ++ wl' ++ wlf in
         run_codegen (compile_instrs mr fe es1) wt wl = inr ((), wt', wl', es') ->
-        ⊢ have_instruction_type_sem rti sr mr M F L1 (wl ++ wl' ++ wlf) (to_e_list es') (InstrT τs1 τs2) L2) ->
-    (forall wt wt' wl wl' wlf es',
+        ⊢ have_instruction_type_sem rti sr mr M F L1 WT WL (to_e_list es') (InstrT τs1 τs2) L2) ->
+    (forall wt wt' wtf wl wl' wlf es',
+        let WT := wt ++ wt' ++ wtf in
+        let WL := wl ++ wl' ++ wlf in
         run_codegen (compile_instrs mr fe es2) wt wl = inr ((), wt', wl', es') ->
-        ⊢ have_instruction_type_sem rti sr mr M F L2 (wl ++ wl' ++ wlf) (to_e_list es') (InstrT τs2 τs3) L3) ->
+        ⊢ have_instruction_type_sem rti sr mr M F L2 WT WL (to_e_list es') (InstrT τs2 τs3) L3) ->
     run_codegen (compile_instrs mr fe (es1 ++ es2)) wt wl = inr ((), wt', wl', es') ->
-    ⊢ have_instruction_type_sem rti sr mr M F L1 (wl ++ wl' ++ wlf) (to_e_list es') (InstrT τs1 τs3) L3.
+    ⊢ have_instruction_type_sem rti sr mr M F L1 WT WL (to_e_list es') (InstrT τs1 τs3) L3.
   Proof.
-    intros fe Hes1 Hes2 Hcompile; rename wl' into wl''.
+    intros fe WT WL Hes1 Hes2 Hcompile; rename wl' into wl''.
     (* Step 1: split out Hcompile into Hcompile_e and Hcompile_es *)
 
     (* For Hcompile_e *)
@@ -2209,22 +2296,27 @@ Section Fundamental.
 *)
   Admitted.
 
-  Lemma compat_instr M F L L' wt wt' wl wl' wlf e ψ es' :
+  Lemma compat_instr M F L L' wt wt' wtf wl wl' wlf e ψ es' :
     let fe := fe_of_context F in
-    (forall wt wt' wl wl' wlf es',
+    let WT := wt ++ wt' ++ wtf in
+    let WL := wl ++ wl' ++ wlf in
+    (forall wt wt' wtf wl wl' wlf es',
        let fe := fe_of_context F in
+       let WT := wt ++ wt' ++ wtf in
+       let WL := wl ++ wl' ++ wlf in
        run_codegen (compile_instr mr fe e) wt wl = inr ((), wt', wl', es') ->
-       ⊢ have_instruction_type_sem rti sr mr M F L (wl ++ wl' ++ wlf) (to_e_list es') ψ L') ->
+       ⊢ have_instruction_type_sem rti sr mr M F L WT WL (to_e_list es') ψ L') ->
     run_codegen (compile_instrs mr fe [e]) wt wl = inr ((), wt', wl', es') ->
-    ⊢ have_instruction_type_sem rti sr mr M F L (wl ++ wl' ++ wlf) (to_e_list es') ψ L'.
+    ⊢ have_instruction_type_sem rti sr mr M F L WT WL (to_e_list es') ψ L'.
   Proof.
-    intros fe IH Hcg.
+    intros fe WT WL IH Hcg.
     unfold compile_instrs, util.mapM_ in Hcg.
     apply wp_ignore in Hcg.
     destruct Hcg as (_ & ? & Hcg).
     apply wp_mapM_cons in Hcg.
     destruct Hcg as ([] & ? & ? & ? & yss_xs & ? & ? & ? & He & Hret & -> & Hwt & Hwl & ->).
     cbn in Hret; inversion Hret; subst; clear Hret.
+    apply IH.
     rewrite -> !app_nil_r in *.
     eauto.
   Qed.
@@ -2416,17 +2508,21 @@ Section Fundamental.
   Qed.
   *)
 
-  Lemma compat_frame M F L L' wt wt' wl wl' wlf es es' τ τs1 τs2 :
+  Lemma compat_frame M F L L' wt wt' wtf wl wl' wlf es es' τ τs1 τs2 :
     let fe := fe_of_context F in
+    let WT := wt ++ wt' ++ wtf in
+    let WL := wl ++ wl' ++ wlf in
     has_mono_rep F τ ->
-    (forall wt wt' wl wl' wlf es',
+    (forall wt wt' wtf wl wl' wlf es',
+        let WT := wt ++ wt' ++ wtf in
+        let WL := wl ++ wl' ++ wlf in
         run_codegen (compile_instrs mr fe es) wt wl = inr ((), wt', wl', es') ->
-        ⊢ have_instruction_type_sem rti sr mr M F L (wl ++ wl' ++ wlf) (to_e_list es') (InstrT τs1 τs2) L') ->
+        ⊢ have_instruction_type_sem rti sr mr M F L WT WL (to_e_list es') (InstrT τs1 τs2) L') ->
     run_codegen (compile_instrs mr fe es) wt wl = inr ((), wt', wl', es') ->
-    ⊢ have_instruction_type_sem rti sr mr M F L (wl ++ wl' ++ wlf) (to_e_list es') (InstrT (τ :: τs1) (τ :: τs2)) L'.
+    ⊢ have_instruction_type_sem rti sr mr M F L WT WL (to_e_list es') (InstrT (τ :: τs1) (τ :: τs2)) L'.
   Proof.
-    intros fe Hmono IH Hcg.
-    eapply (IH _ _ _ _ wlf) in Hcg.
+    intros fe WT WL Hmono IH Hcg.
+    eapply (IH _ _ _ _ _ wlf) in Hcg.
     unfold have_instruction_type_sem.
     iIntros (s__mem s__rep s__size se inst fr lh rvs vs' Henv) "Hinst Hctx Hrvs Hvs Hfr Hf Hrun".
     (*
@@ -2446,26 +2542,31 @@ Section Fundamental.
     *)
   Admitted.
 
-  Theorem fundamental_theorem M F L L' wt wt' wl wl' wlf es es' tf :
+  Theorem fundamental_theorem M F L L' wt wt' wtf wl wl' wlf es es' tf :
     have_instruction_type M F L es tf L' ->
     let fe := fe_of_context F in
+    let WT := wt ++ wt' ++ wtf in
+    let WL := wl ++ wl' ++ wlf in
     run_codegen (compile_instrs mr fe es) wt wl = inr (tt, wt', wl', es') ->
-    ⊢ have_instruction_type_sem rti sr mr M F L (wl ++ wl' ++ wlf) (to_e_list es') tf L'.
+    ⊢ have_instruction_type_sem rti sr mr M F L WT WL (to_e_list es') tf L'.
   Proof.
     intros Htype.
     generalize dependent es'.
     generalize dependent wlf.
     generalize dependent wl'.
     generalize dependent wl.
+    generalize dependent wtf.
     generalize dependent wt'.
     generalize dependent wt.
     induction Htype using have_instruction_type_mind with
       (P1 := fun M F L e ψ L' =>
-               forall wt wt' wl wl' wlf es',
+               forall wt wt' wtf wl wl' wlf es',
                  let fe := fe_of_context F in
+                 let WT := wt ++ wt' ++ wtf in
+                 let WL := wl ++ wl' ++ wlf in
                  run_codegen (compile_instr mr fe e) wt wl = inr (tt, wt', wl', es') ->
-                 ⊢ have_instruction_type_sem rti sr mr M F L (wl ++ wl' ++ wlf) (to_e_list es') ψ L');
-      intros wt wt' wl wl' wlf wes fe Hcomp.
+                 ⊢ have_instruction_type_sem rti sr mr M F L WT WL (to_e_list es') ψ L');
+      intros wt wt' wtf wl wl' wlf wes fe WT WL Hcomp.
     - eapply compat_nop; eassumption.
     - eapply compat_unreachable; eassumption.
     - eapply compat_copy; eassumption.
